\section{Denotational semantics}

We now build on Proposition~\ref{prop:expressions} to prove the denotational
results claimed at the start of the paper.  

Recall that we write $P[T]$ for the process~$P$ interpreted in the script
where the distinguished type~|T| is given value~$T$.  We make this more
precise.  Recall that we write $\rho^T$ for the environment that results from
evaluating just the declaration of~|T| with value~$T$
(Definition~\ref{def:initial-env}).  Suppose $decls$ represents the top-level
declarations in the script.  Then the environment formed from these
declarations is $\bindDecls \rho^{T_1}~decls$.  So the value of~$P$ in the
script is
\begin{eqnarray*}
P[T] & \defs &  \eval (\bindDecls \rho^{T}~decls)~P.
\end{eqnarray*}
%
The following lemma relates the value of~$P$ in the two different scripts.
%
\begin{lemma}
Let $f: T_1 \fun T_2$ be surjective.  Then $P[T_2] = f(P[T_1])$. 
\end{lemma}
%
\begin{proof}
\begin{calc}
& P[T_2] \\
= & \eval (\bindDecls \rho^{T_2}~decls)~P \\
= & \com{Lemma~\ref{lem:distinguished-type-declaration}} \\
  & \eval (\bindDecls (f(\rho^{T_1}))~decls) ~P \\
= & \com{clause~\ref{item:bindDecls} of Proposition~\ref{prop:expressions}} \\
  & \eval (f(\bindDecls \rho^{T_1}~decls)) ~P \\
= & \com{clause~\ref{item:eval}  of Proposition~\ref{prop:expressions}} \\
  & f( \eval (\bindDecls \rho^{T_1}~decls)) ~P \\
= & f(P[T_1]) .
\end{calc}
\end{proof}

It immediately follows that for each transition of $P[T_1]$ using event~$a$,
there is a corresponding transition of~$P[T_2]$ using event $f(a)$.  
%
\begin{lemma}
If
\[
(P,\rho) \trans{a} (Q,\rho_2)  \quad \mbox{in $P[T_1]$}\,,
\]
then
\[
(P,f(\rho)) \trans{f(a)} (Q,f(\rho_2))  \quad \mbox{in $P[T_2]$}.
\]
\end{lemma}

The proof of the converse is made more difficult by the fact that applying~$f$
to $\eval \rho~P$ can merge states.  A particular state $(Q,\rho_1)$ gets
mapped to $(Q,f(\rho_1))$, but so does any other state $(Q,\rho_2)$ such that
$f(\rho_2) = f(\rho_1)$.  The resulting state has transitions corresponding to
the union of the transitions from $(Q,\rho_1)$ and $(Q,\rho_2)$ (remapped
by~$f$).  We need to show that each transition of $(Q,f(\rho_1))$ does
correspond to a transition of~$(Q,\rho_1)$. 

%% \begin{lemma}
%% Suppose $(Q, \rho)$ is a state in $P[T_1]$, and suppose there is a transition
%% \[
%% (Q, f(\rho)) \trans{a} (Q',\rho_1)  \quad \mbox{in $P[T_2] = f(P[T_1])$.}
%% \]
%% Then there is a transition 
%% \[
%% (Q, \rho) \trans{a'} (Q', \rho_1') \quad \mbox{in $P[T_1]$}
%% \]
%% such that $f(a') = a$, and $f(\rho_1') = \rho_1$.
%% \end{lemma}

%% \begin{proof}
%% The sub-ALTS rooted at $(Q,\rho)$ and $(Q, f(\rho))$ are equal to $\eval \rho~Q$
%% and $\eval Q f(\rho)~Q = f(\eval \rho~Q)$, respectively.  

%% , by
%% Proposition~\ref{prop:expressions}.  

%% \end{proof}



%%%%%%%%%%%%%%%%%%%%%%%%%%%%%%%%%%%%%%%%%%%%%%%%%%%%%%%

\subsection{Ignore?? }



%
The following sequence of lemmas proves the converse.
%
\begin{lemma}
\label{lem:f-sim-expr}
Suppose $f(\rho) = f(\rho')$.  Then for every expression~$e$,\,
\[
f(\eval \rho~e) =f(\eval \rho'~e).
\]
\end{lemma}
%
\begin{proof}
We have
\(
f(\eval \rho~e) = \eval (f(\rho))~e = \eval (f(\rho'))~e = f(\eval \rho'~e)
\),
using Proposition~\ref{prop:expressions}.
\end{proof}

%%%%%%%%%%

\begin{lemma}
\label{lem:f-sim-proc}
Consider two ALTS states $(Q,\rho)$ and $(Q,\rho')$ such that $f(\rho) =
f(\rho')$.  Suppose there is a transition
\[
(Q,\rho) \trans{a} (Q',\rho_1),
\]
Then there is also a transition
\[
(Q,\rho') \trans{a'} (Q',\rho_1'),
\]
such that $f(a) = f(a')$ and $f(\rho_1) = f(\rho_1')$.
\end{lemma}
%
\begin{proof}
The ALTSs rooted at the two states are equal to $\eval \rho ~ Q$ and $\eval
\rho'~ Q$, respectively.  By Lemma~\ref{lem:f-sim-expr}, $f(\eval \rho~ Q) =
f(\eval \rho' ~Q)$.  Then \framebox{????}
\end{proof}


%%%%%%%%%%%%%%%%%%%%%%%%%%%%%%%%%%%%%%%%%%%%%%%%%%%%%%%

%% Consider, the case of a process expression~$P$.  Recall that $\eval \rho~P$ is
%% an ALTS with initial state~$(P,\rho)$; we write $ALTS_{P,\rho}$ for this
%% ALTS\@.  The following lemma follows immediately from
%% Lemma~\ref{lem:f-sim-expr}.
%% %
%% \begin{lemma}
%% \label{lem:f-sim-proc}
%% Suppose $f(\rho) = f(\rho')$.  Then $f(ALTS_{P,\rho}) = f(ALTS_{P,\rho'})$.
%% In particular, for every transition 
%% \[
%% (P,\rho) \trans{a} (Q,\rho_2)  \quad \mbox{in $ALTS_{P,\rho}$}\,,
%% \]
%% there is a corresponding transition 
%% \[
%% (P,\rho') \trans{a'} (Q,\rho_2')  \quad \mbox{in $ALTS_{P,\rho'}$}
%% \]
%% such that $f(a) = f(a')$, and $f(\rho_2) = f(\rho_2')$, and vice versa.
%% \end{lemma}


%%%%%%%%%%

\begin{lemma}
Suppose $(Q, \rho)$ is a state in $P[T_1]$, and suppose there is a transition
\[
(Q, f(\rho)) \trans{a} (Q',\rho_1)  \quad \mbox{in $P[T_2] = f(P[T_1])$.}
\]
Then there is a transition 
\[
(Q, \rho) \trans{a'} (Q', \rho_1') \quad \mbox{in $P[T_1]$}
\]
such that $f(a') = a$, and $f(\rho_1') = \rho_1$.
\end{lemma}

\framebox{XXX}

I don't think the above holds from what I've proved so far.  Consider a
process~$Q$ equivalent to $\If x = y \Then a \then STOP \Else STOP$, and let
$\rho = \set{x \mapsto A, y \mapsto B}$.  Then $(Q,\rho)$ does not have a
transition on~$a$.  But if $f(A) = f(B) = C$, then $(Q,f(\rho))$ does have a
transition on~$a$.  This doesn't contradict Proposition~\ref{prop:expressions}
as written, because $f$ merges $(Q,\rho)$ with $(Q,\rho')$ where $\rho' =
\set{x \mapsto A, y \mapsto B}$, which does have a transition on~$a$. 


\begin{proof}
The transition in $f(P[T_1])$ results from the application of~$f$ to a
transition in $P[T_1]$; that transition must be of the form
\[
(Q, \rho') \trans{a''} (Q', \rho'') % \quad \mbox{in $ALTS_{P,\rho}$}
\]
such that $f(\rho') = f(\rho)$,\, $f(a'') = a$, and $f(\rho'') = \rho_1$.
Then Lemma~\ref{lem:f-sim-proc} implies the existence of a transition
\[
(Q, \rho) \trans{a'} (Q', \rho_1') % \quad \mbox{in $ALTS_{P,\rho}$}
\]
such that $f(a') = f(a'') = a$, and $f(\rho_1') = f(\rho'') = \rho_1$, as
required. 
\end{proof}





%%%%%%%%%%%%%%%%%%%%%%%%%%%%%%%%%%%%%%%%%%%%%%%%%%%%%%%


%% Suppose  there is a transition 
%% \[
%% (Q_1,\rho_1) \trans{a} (Q_2,\rho_2) \quad \mbox{in $f(ALTS_{P,\rho})$.}
%% \]
%% Then there is a transition
%% \[
%% (Q_1,\rho_1') \trans{a'} (Q_2,\rho_2') \quad \mbox{in $ALTS_{P,\rho}$}
%% \]
%% such that $f(\rho_1') = \rho_1$,\, $f(a') = a$, and $f(\rho_2') = \rho_2$.
%% Suppose also $f(\rho_1'') = f(\rho_1') = \rho_1$.  Then
%% there is a transition
%% \[
%% (Q_1,\rho_1'') \trans{a''} (Q_2,\rho_2'') \quad \mbox{in $ALTS_{P,\rho}$}
%% \]
%% such that $f(a'') = f(a') = a$ and $f(\rho_2'') = f(\rho_2') = \rho_2$.

Not apply induction.
